Source/IntegrationTests/TestFiles/LitTests/LitTest/comp/rust/classes.dfy
@@ -1,0 +1,21 @@
+// RUN: %baredafny translate rs %args "%s"
+// RUN: %OutputCheck --file-to-check "%S/classes-rust/src/classes.rs" "%s"
+// CHECK: y: .*MaybeUninit
+// RUN: %baredafny run --target=rs > "%t"
+// RUN: %diff "%s.expect" "%t"
+
+class Y {
+  var c: int
+}
+class X {
+  var y: Y
+  constructor() {
+    y := new Y;
+    new;
+    y.c := 0;
+  }
+}
+method Main() {
+  var x := new X();
+  print x.y.c;
+}
